# math410; 02.05.2025

## Proving convergence

*Limit Notation for convergence:*
$$
\lim_{n \rightarrow \infty} a_n = L
$$
*Example:* Want to show $\set{ \frac{(-1)^n}{n} }$ converges to $0$. That is, $\lim_{n \rightarrow \infty} \frac{(-1)^n}{n} = 0$.

- **Proof:**

  Let $\epsilon > 0$ be given. 

  By A.P., $\exists N \in \mathbb{N}$ such that $\frac{1}{\epsilon} < N$. Rearranging, we find $\frac{1}{N} < \epsilon$.

  Then for $n \geq N$, 
  $$
  |a_n - L| = \left|\frac{(-1)^n}{n} - 0\right| = \frac{1}{n} \leq \frac{1}{N} < \epsilon
  $$
  as needed. 
  $$
  \begin{align*}
  	\lim_{n \rightarrow \infty} \frac{(-1)^n}{n} 
  		&= 0 
  		&\square
  \end{align*}
  $$
  

*Example:* Prove that $\set{ \frac{n^2 - 2n}{n^2 + 1} }$ converges to $1$.

- That is, $\lim_{n \rightarrow 0} \frac{n^2 - 2n}{n^2 + 1} = 1$.

- **Proof:**

  Let $\epsilon > 0$ be given. 

  By A.P., $\exists N \in \mathbb{N}$ such that $\frac{3}{\epsilon} < N$. $\forall n > N$,
  $$
  \begin{align*}
  	|a_n - L| 
  		&= \left| \frac{n^2 - 2n}{n^2 + 1} - 1 \right| \\
  		&= \left| \frac{-2n - 1}{n^2 + 1} \right| \\
  		&= |-1| \cdot \frac{|2n + 1|}{|n^2 + 1|}\\
  		&= \frac{2n + 1}{n^2 + 1} \\
  		&\leq \frac{3n}{n^2 + 1} \leq \frac{3n}{n^2} \\ 
  		&= \frac{3}{n} \leq \frac{3}{N} \\
  		&\leq 3\cdot \frac{\epsilon}{3} = \epsilon,
  \end{align*}
  $$
  as needed.
  $$
  \begin{align*}
  	\lim_{n \rightarrow 0} \frac{n^2 - 2n}{n^2 + 1} &= 1 &\square
  \end{align*}
  $$