# math410; 03.05.2025

## Exam review in class

### Practice problems.

1. Suppose sequence $a_n$ is bounded and sequence $b_n$ diverges to $\infty$. Prove that $b_n$ diverges to $\infty$.

   **Proof.**

   Let $\{a_n\}$ be bounded, then $\exists M \in \mathbb{R^+}$ such that $|a_n| \leq M, \forall n$. Then,
   $$
   -M \leq a_n \leq M , \quad \forall n
   $$
   

   Let $C > 0$ be given. By def'n of divergence, $\exists N \in \mathbb{N}$ such that $b_n > C + M$ for all $n \geq N$.

   For $n \geq N$,
   $$
   \begin{align*}
   	a_n + b_n \geq -M + b_n > -M + C + M = C.
   \end{align*}
   $$
   So we have $a_n + b_n > C$ for $n \geq N$, as needed. $\square$

   ---

2. Using the definition of a limit, find the limit of the sequence
   $$
   a_n = \frac{2n + 1}{n - 1} + \frac{1}{n}.
   $$
   **Proof.**

   > Intuitively, we know the first term goes to two and the second term goes to zero. So we know the limit is $2$.

   Let $\epsilon > 0$ be given. By A.P., $\exists N \in \mathbb{N}$ such that $N > 1 + \frac{4}{\epsilon} \in \mathbb{R^+}$.

   Then for all $n \geq N$,
   $$
   \begin{align*}
   	|\frac{2n + 1}{n - 1} + \frac{1}{n} - 2| 
   		&= |\frac{n(2n + 1) + (n - 1) - 2n(n - 1)}{n(n - 1) }| \\
   		&= |\frac{2n^2 + 2n - 1 - 2n^2 + 2n}{n(n - 1)}| \\
   		&= |\frac{4n - 1}{n(n - 1)}| 
   			< |\frac{4n}{n(n - 1)}| 
   				= |\frac{4}{n - 1}| \\
           &= \frac{4}{n - 1} < \frac{4}{N - 1} = \epsilon,
   \end{align*}
   $$
   as needed. So we have $\{a_n\} \rightarrow 2$. $\square$

   ---

3. Skipped.

4. Prove the function $f(x) = \frac{1}{x^2}$ on $(0, \infty)$ satisfies the $\epsilon - \delta$ criterion for continuity.

   **Proof.** 

   Let $x_0 \in (0, \infty)$ and $\epsilon > 0$ be given.

   $f$ would fulfill the $\epsilon - \delta$ continuity criterion if $\exists \delta > 0$ such that if $|x - x_0| < \delta$, then $|f(x) - f(x_0)| < \epsilon$.

   Let $\delta = \frac{x_0}{2}$. Then,
   $$
   \begin{align*}
   	|x - x_0| &< \delta = \frac{x_0}{2} \\
   	-\frac{x_0}{2} &< x - x_0 < \frac{x_0}{2} \\
   	0< \frac{x_0}{2} < x &< \frac{3x_0}{2}. \\
   	\text{Then } \frac{x_0}{2} &< |x| < \frac{3x_0}{2}.
   \end{align*}
   $$
   Assume if $|x - x_0| < \delta$, then
   $$
   \begin{align*}
   	|f(x) - f(x_0)| 
   		&= |\frac{1}{x^2} - \frac{1}{x_0^2}| \\
   		&= |\frac{x_0^2 - x^2}{x^2 x_0^2}| \\
   		&= \frac{|x_0 + x| \cdot |x_0 - x|}{|x^2| \cdot |x_0^2|} \\
   		&< \delta \frac{|x_0 + x|}{|x^2| |x_0^2|} \\
   		&< \delta \frac{x_0 + e}{}
   \end{align*}
   $$