# math410; 03.10.2025

## Differentiation

### Defining the derivative

Take the secant line from one point $x_0$ to another point $x$, and let $x \rightarrow x_0$. So the limit of the secant line between $x_0$ and $x$ as $x \rightarrow x_0$.

Take a sequence of secant lines closer to $x$,
$$
\lim_{x \rightarrow x_0} \frac{f(x) - f(x_0)}{x - x_0}.
$$
We now go to define it formally.

- For $x_0 \in \mathbb{R}$, the open interval $I = (a, b)$ that contains $x_0$ is called a **neighborhood** of $x_0$.

  Then, $f: I \rightarrow \mathbb{R}$ is **differentiable at $x_0$** if
  $$
  \lim_{x \rightarrow x_0} \frac{f(x) - f(x_0)}{x - x_0} = f'(x_0) \text{ exists,}
  $$
  where $f'(x_0)$ is the **derivative at point $x_0$**.

  If $f$ is differentiable at all points in $I$, then we say generally:

  - $f$ is **differentiable**.
  - $f' : I \rightarrow \mathbb{R}$ is the **derivative**.

### Derivatives of polynomials

**Example.** Let $f(x) = mx + b$. Find $f'(x_0)$.

- Let $x \in D - \{x_0\}$. Then,
  $$
  \begin{align*}
  	f'(x_0) 
  		&= \lim_{x \rightarrow x_0} \frac{f(x) - f(x_0)}{x - x_0} \\
  		&= \lim_{x \rightarrow x_0} \frac{mx + b - mx_0 - b}{x - x_0} \\
  		&= \lim_{x \rightarrow x_0} \frac{m(x - x_0)}{x - x_0} = m.
  \end{align*}
  $$
  So $f'(x_0) = m$.

**Example.** Let $f(x) = x^2$. Find $f'(x_0)$.

- Let $x \in D - \{x_0\}$. Then,
  $$
  \begin{align*}
  	f'(x_0) 
  		&= \lim_{x \rightarrow x_0} \frac{f(x) - f(x_0)}{x - x_0} \\
  		&= \lim_{x \rightarrow x_0} \frac{x^2 - x_0^2}{x - x_0} \\
  		&= \lim_{x \rightarrow x_0} \frac{(x + x_0)(x - x_0)}{x - x_0} \\
  		&= \lim_{x \rightarrow x_0} (x + x_0) \\
  		&= x_0 + x_0 = 2x_0.
  \end{align*}
  $$
  So $f'(x_0) = 2x_0$.

**Example.** Let $f(x) = x^n$. Find $f'(x_0)$.

- Let $x \in D - \{x_0\}$. Then,
  $$
  \begin{align*}
  	f'(x_0)
  		&= \lim_{x \rightarrow x_0} \frac{f(x) - f(x_0)}{x - x_0} \\
  		&= \lim_{x \rightarrow x_0} \frac{x^n - x_0^n}{x - x_0} \\
      \text{Recall that } x^n - x_0^n 
      	&= (x - x_0) (x^{n - 1} + x^{n - 2} x_0 + \cdots + x x_0^{n - 2} + x_0^{n - 1}) \\
      	\text{So } f'(x_0) &= \lim_{x \rightarrow x_0} [x^{n - 1} + x^{n - 2} x_0 + \cdots + x x_0^{n - 2} + x_0^{n - 1}] \\
      	&= x_0^{n - 1} + x_0^{n - 2} x_0 + \cdots + x_0 x_0^{n - 2} + x_0^{n - 1} \\
      	&= x_0^{n - 1} + x_0^{n - 1} + \cdots + x_0^{n - 1} + x_0^{n - 1}
      		&\text{$n$ terms} \\
          &= n x_0^{n - 1}.
  \end{align*}
  $$
  So $f'(x_0) = n x^{n - 1}$. We have shown this for $n \in \mathbb{N}$. We know from Calculus I that it works for fractional powers, this will be proven later.

### Differential $\rightarrow$ continuous

**Theorem.** If $f: I \rightarrow \mathbb{R}$ is *differentiable* at $x_0$, then $f$ is also continuous at $x_0$.

> [!WARNING]
>
> Note that this is **not** an *if and only if*. There are plenty counterexamples where a continuous $f$ is not differentiable, like $|x|$ at $x = 0$ is a cusp/sharp point with no derivative, despite $|x|$ being continuous everywhere.

- **Proof.** Let $x \in I$ where $x \neq x_0$.

  Since $f$ is differentiable at $x_0$, then
  $$
  f'(x_0) = \lim_{x \rightarrow x_0} \frac{f(x) - f(x_0)}{x - x_0} \text{ exists}.
  $$
  We will use this to show continuity.
  $$
  \text{Let } \lim_{x \rightarrow x_0} [x - x_0] = 0.
  $$
  Then, we consider $f(x) - f(x_0)$:
  $$
  \begin{align*}
  	\lim_{x \rightarrow x_0} [f(x) - f(x_0)]
  		&= \lim_{x \rightarrow x_0} (x - x_0) \cdot \frac{f(x) - f(x_0)}{x - x_0} \\
  		&= 0 \cdot f'(x_0) = 0,
  			&\text{product prop. of limits}
  \end{align*}
  $$
  as needed! $\square$

### Properties of derivatives

**Sum, product, and quotient properties.** If $f: I \rightarrow \mathbb{R}$ and $g: I \rightarrow \mathbb{R}$ are differentiable at $x_0$, then
$$
\begin{align}
	(f \pm g)' (x_0) &= f'(x_0) + g'(x_0) 
		&\text{(I)} \\
	(f g)' (x_0) &= f'(x_0) g(x_0) + f(x_0) g'(x_0)
    	&\text{(II)} \\
    \left(\frac{f}{g}\right)'(x_0) &= \frac{f'(x_0) g(x_0) - f(x_0) g'(x_0)}{[g(x_0)]^2}
    	&\text{(III)} \\
\end{align}
$$

- **Proof of I.**
  $$
  \begin{align*}
  	(f \pm g)'(x_0) 
  		&= \lim_{x \rightarrow x_0} \frac{(f \pm g)(x) - (f \pm g)(x_0)}{x - x_0} \\
  		&= \lim_{x \rightarrow x_0} \frac{f(x) - f(x_0)}{x - x_0}
  			\pm \lim_{x \rightarrow x_0} \frac{g(x) - f(g_0)}{x - x_0} \\
          &= f'(x_0) + g'(x_0).
  \end{align*}
  $$

- **Proof of II.**
  $$
  \begin{align*}
  	(fg)'(x_0) 
  		&= \lim_{x \rightarrow x_0} \frac{(fg)(x) - (fg)(x_0)}{x - x_0} \\
  		&= \lim_{x \rightarrow x_0} \frac{f(x)g(x) - f(x_0)g(x_0)}{x - x_0} \\
  		&= \lim_{x \rightarrow x_0} \frac{f(x)g(x) - f(x_0)g(x) + f(x_0)g(x) - f(x_0)g(x_0)}{x - x_0} \\
  		&= \lim_{x \rightarrow x_0} \frac{g(x)[f(x) - f(x_0)] 
  			+ f(x_0)[g(x) - g(x_0)]}{x - x_0} \\
  		&= \lim_{x \rightarrow x_0} g(x) \frac{f(x) - f(x_0)}{x - x_0}
  			+ \lim_{x \rightarrow x_0} f(x_0) \frac{g(x) - g(x_0)}{x - x_0} \\
          &= g(x_0) f'(x_0) + f(x_0) g'(x_0)
          	&\text{$g$ is cont. since its diff} \\
          	&&\text{by 3.7, $\lim_{x \rightarrow x_0} g(x) = g(x_0)$}
  \end{align*}
  $$
  