# math462; 03.03.2025

## Heat equation, cont'd

### Error function

We say that expressions of the form
$$
\int_{0}^{x} e^{-p^2} dp
$$
are called **error functions**.

More specifically, we define the "error function" by
$$
\text{Erf} (x) = \frac{2}{\sqrt{\pi}} \int_{0}^{x} e^{-p^2}\, dp.
$$
Observe things about this function:
$$
\begin{align*}
	\frac{d}{dx} [\text{Erf} (x)] 
		&= \frac{2}{\sqrt{\pi}} e^{-x^2} \ \\
	\lim_{x \rightarrow \infty} \text{Erf}(x) = 1, 
		&\quad \lim_{x \rightarrow -\infty} \text{Erf}(x) = -1 \\
    \text{Erf is odd:} &\quad \text{Erf}(-x) = -\text{Erf}(x)
\end{align*}
$$

### General solution to heat equation

Last class, we saw that $Q$, when $Q_t = k Q_{xx}$ with $\lim_{t \rightarrow 0^{+}} Q(x, t) = H(x)$, was
$$
\begin{align*}
	Q(x, t) 
		&= \frac{1}{2} + \frac{1}{\sqrt{\pi}} \int_{0}^{\frac{x}{4kt}} e^{-p^2} dp \\
    	&= \frac{1}{2} + \frac{1}{2} \,\text{Erf}(x).
\end{align*}
$$
We defined $S = \frac{\partial Q}{\partial x}$ to be
$$
S(x, t) = \frac{1}{\sqrt{4\pi kt}} e^{-\frac{x^2}{4kt}}.
$$
**Theorem:** 

- Solution of
  $$
  u_t = k u_{xx} \qquad (-\infty < x < \infty \quad t > 0)
  $$
  with initial condition $\lim_{t \rightarrow 0^{+}} u(x, t) = \phi(x)$ is
  $$
  u(x, t) = \frac{1}{\sqrt{4 \pi k t}} \int_{-\infty}^{\infty} \phi(y) dy.
  $$
  This can be expressed also as
  $$
  \int_{-\infty}^{\infty} S(x - y, t) \, \phi (y) \, dy.
  $$

A common substitution: $p = \frac{y - x}{\sqrt{4kt}}$. Then,

- $dp = \frac{1}{\sqrt{4kt}} dy$. So we have,
  $$
  u(x, t) = \frac{1}{\pi} \int_{\infty}^{\infty} e^{-p^2} \, \phi(x + p \sqrt{4kt}) \, dp.
  $$
  This form *may or may not* be nicer; context dependent.

### Examples

We have an infinite rod. Let $u_t = k u_{xx}$, where $-\infty < x < \infty$ and $t > 0$, with initial condition
$$
\phi(x) = \begin{cases}
	1 &\text{if } -1 < x < 1 \\
	0 &\text{if } |x| \geq 1
\end{cases}
$$

- **Solution.**
  $$
  \begin{align*}
  	u(x, t) 
  		&= \frac{1}{\sqrt{4 \pi k t}} \int_{-\infty}^{\infty} e^{-\frac{(x - y)^2}{4kt}}\,\phi(y)\,dy \\
  		&= \frac{1}{\sqrt{4 \pi k t}} \int_{-1}^{1} e^{-\frac{(x - y)^2}{4kt}}\,(1)\,dy \\
  		&= \frac{1}{\sqrt{4 \pi k t}} \int_{-1}^{1} e^{-\frac{(x - y)^2}{4kt}}\,dy
  \end{align*}
  $$
  As an exercise, we try and rewrite in terms of $\text{Erf}$:
  $$
  \begin{align*}
  	\text{Let } p &= \frac{y - x}{\sqrt{4kt}} \\
  	dp &= \frac{1}{\sqrt{4kt}} dy \\
  	\text{As }y \rightarrow 1,&\quad p \rightarrow \frac{1 - x}{\sqrt{4kt}} \\
  	\text{As }y \rightarrow -1,&\quad p \rightarrow \frac{-1 -x}{\sqrt{4kt}}
  \end{align*}
  $$
  Then we substitute into the integral in $u$:
  $$
  \begin{align*}
  	u(x, t) 
  		&= \frac{1}{\pi} \int_{\frac{-1 -x}{\sqrt{4kt}}}^{\frac{1 -x}{\sqrt{4kt}}} e^{-p^2} dp \\
  		&= \frac{1}{\pi} \left[\int_{0}^{\frac{1 -x}{\sqrt{4kt}}} e^{-p^2} dp  
  			+ \int_{\frac{-1 -x}{\sqrt{4kt}}}^{0} e^{-p^2} dp \right] \\
          &= \frac{1}{2} \text{Erf} \left(\frac{1 - x}{\sqrt{4kt}} \right) 
          	+ \frac{1}{\pi} \int_{\frac{-1 -x}{\sqrt{4kt}}}^{0} e^{-p^2} dp \\
          &= \frac{1}{2} \text{Erf} \left(\frac{1 - x}{\sqrt{4kt}} \right) 
          	- \frac{1}{\pi} \int_{0}^{\frac{-1 -x}{\sqrt{4kt}}} e^{-p^2} dp \\
          &= \frac{1}{2} \text{Erf} \left(\frac{1 - x}{\sqrt{4kt}} \right)  - \frac{1}{2} \text{Erf} \left(\frac{-1 - x}{\sqrt{4kt}} \right) 
  \end{align*}
  $$

**Consider** $u_t = k u_{xx}$ where $-\infty < x < \infty$ and $t > 0$, with the initial condition of $\phi(x) = e^x$.

- **Solution.** Substitute into general equation.
  $$
  \begin{align*}
  	u(x, t) 
  		&= \frac{1}{\sqrt{4 \pi kt}} \int_{-\infty}^{\infty} e^{-\frac{(x - y)^2}{4kt}}\, e^y \, dy \\
  		&= \frac{1}{\sqrt{4 \pi kt}} \int_{-\infty}^{\infty}  e^{- \frac{(x - y)^2}{4kt} + y} \, dy \\
  \end{align*}
  $$
  We can "complete the square" to simplify the exponent.
  $$
  \begin{align*}
  	- \frac{(x - y)^2}{4kt} + y
  		&= -\frac{1}{4kt} (y + 2kt - x)^2 + kt + x
  \end{align*}
  $$
  Then,
  $$
  \begin{align*}
  	u(x, t) &= \frac{1}{\sqrt{4 \pi kt}} \int_{-\infty}^{\infty} e^{-\frac{1}{4kt} (y + 2kt - x)^2 + kt + x}
  \end{align*}
  $$
  
  Incomplete...

